theories/L2_5_box/L2_5.v
@@ -1,0 +1,4 @@
+(** Collect all of L2_5 together **)
+
+Require Export L2_5.compile.
+Require Export L2_5.term L2_5.program L2_5.wndEval L2_5.wcbvEval L2_5.wNorm.
