theories/L2_5_box/stripEvalCommute.v
@@ -1,0 +1,118 @@
+Require Import Coq.Lists.List.
+Require Import Coq.Strings.String.
+Require Import Coq.Strings.Ascii.
+Require Import Coq.Arith.Compare_dec.
+Require Import Coq.Arith.Peano_dec.
+Require Import Coq.Setoids.Setoid.
+Require Import Omega.
+
+Require Import L2.L2.
+Require Import L2_5.compile.
+Require Import L2_5.term.
+Require Import L2_5.program.
+Require Import L2_5.wndEval.
+Require Import L2_5.wcbvEval.
+
+Local Open Scope string_scope.
+Local Open Scope bool.
+Local Open Scope list.
+Set Implicit Arguments.
+
+Definition L2Term := L2.compile.Term.
+Definition L2Terms := L2.compile.Terms.
+Definition L2Defs := L2.compile.Defs.
+Definition strip := L2Term_Term.
+Definition strips := L2Terms_Terms.
+Definition stripDs := L2Defs_Defs.
+Definition stripEnv := L2Env_Env.
+Definition stripEc := L2EC_EC.
+
+Definition optStrip (t:option L2Term) : option Term :=
+  match t with
+    | None => None
+    | Some t => Some (strip t)
+  end.
+Definition optStrips (ts:option L2Terms) : option Terms :=
+  match ts with
+    | None => None
+    | Some ts => Some (strips ts)
+  end.
+Definition optStripDnth (b: option (L2Term * nat)) : option (Term * nat) :=
+                           match b with
+                             | None => None
+                             | Some (t, n) => Some (strip t, n)
+                           end.
+Definition optStripCanP
+           (b: option (nat * L2Terms * nat)): option (nat * Terms * nat) :=
+                           match b with
+                             | None => None
+                             | Some (n, t, m) => Some (n, strips t, m)
+                           end.
+
+Lemma optStrip_hom: forall y, optStrip (Some y) = Some (strip y).
+induction y; simpl; reflexivity.
+Qed.
+Lemma optStrips_hom: forall y, optStrips (Some y) = Some (strips y).
+induction y; simpl; reflexivity.
+Qed.
+Lemma optStripDnth_hom:
+  forall y n, optStripDnth (Some (y, n)) = Some (strip y, n).
+induction y; simpl; reflexivity.
+Qed.
+Lemma optStripCanP_hom:
+  forall y n m, optStripCanP (Some (n, y, m)) = Some (n, strips y, m).
+induction y; simpl; reflexivity.
+Qed.
+                              
+Print L2Env.
+Lemma Lookup_hom:
+  forall (p:environ L2.compile.Term) s ec, Lookup s p ec -> Lookup s (L2Env_Env p) (L2EC_EC ec).
+Proof.
+  induction 1; destruct t.
+  - change (Lookup s ((s, ecTrm (strip t)) :: (L2Env_Env p))
+                   (ecTrm (strip t))).
+    apply LHit.
+  - cbn. apply LHit.
+  - change (Lookup s2 ((s1, ecTrm (strip t)) :: (L2Env_Env p))
+                   (L2EC_EC ec)).
+    apply LMiss; assumption.
+  - cbn. apply LMiss; assumption.
+Qed.
+
+Lemma LookupDfn_hom:
+ forall p s t, LookupDfn s p t -> LookupDfn s (stripEnv p) (strip t).
+unfold LookupDfn. intros.
+assert (j:= Lookup_hom H). exact j.
+Qed.
+
+Lemma dlength_hom:
+  forall ds, L2.term.dlength ds = dlength (stripDs ds).
+induction ds. intuition. simpl. rewrite IHds. reflexivity.
+Qed.
+
+Lemma tcons_hom:
+  forall t ts, strips (L2.compile.tcons t ts) = tcons (strip t) (strips ts).
+reflexivity.
+Qed.
+
+Lemma tnil_hom: strips L2.compile.tnil = tnil.
+reflexivity.
+Qed.
+
+Lemma dcons_hom:
+  forall nm bod rarg ds,
+    stripDs (L2.compile.dcons nm bod rarg ds) =
+    dcons nm (strip bod) rarg (stripDs ds).
+reflexivity.
+Qed.
+
+Lemma dnil_hom: stripDs L2.compile.dnil = dnil.
+reflexivity.
+Qed.
+
+Lemma dnthBody_hom: 
+  forall m ds, optStripDnth (L2.term.dnthBody m ds) =
+               dnthBody m (stripDs ds).
+induction m; induction ds; try intuition.
+- simpl. intuition.
+Qed.
