theories/L2_5_box/stripWndCommute.v
@@ -1,0 +1,19 @@
+
+Require Import Coq.Lists.List.
+Require Import Coq.Strings.String.
+Require Import Coq.Strings.Ascii.
+Require Import Coq.Arith.Compare_dec.
+Require Import Coq.Arith.Peano_dec.
+Require Import Coq.Setoids.Setoid.
+Require Import Omega.
+
+Require Import L2.L2.
+Require Import L2_5.program.
+Require Import L2_5.wndEval.
+Require Import L2_5.stripEvalCommute.
+Require Import L2_5.term.
+Require Import L2_5.compile.
+
+Definition L2Term := L2.compile.Term.
+Definition L2Terms := L2.compile.Terms.
+Definition L2Defs := L2.compile.Defs.
