theories/L2_typeStripped/L2.v
@@ -4,4 +4,5 @@ Add LoadPath "../L2_typeStripped" as L2.
 
 Require Export L2.compile.
 Require Export L2.term L2.program L2.wndEval L2.wcbvEval L2.wNorm.
-Require Export L2.stripEvalCommute.
+Require Export L2.stripEvalCommute L2.stripWndCommute.
+
